coq/Desc.v
@@ -1,0 +1,79 @@
+
+Class Desc (From : Type) :=
+  {
+    To : Type;
+    denote : From -> To;
+  }.
+
+Notation "⟦ d ⟧" := (denote d).
+
+Inductive TypeD : Type :=
+| ArrowD : TypeD -> TypeD -> TypeD
+| BoolD  : TypeD
+| ListD  : TypeD -> TypeD
+| NatD   : TypeD
+.
+
+Fixpoint denoteTypeD d :=
+  match d with
+  | ArrowD dL dR => denoteTypeD dL -> denoteTypeD dR
+  | BoolD        => bool
+  | ListD  dT    => list (denoteTypeD dT)
+  | NatD         => nat
+  end.
+
+Global Instance Desc_TypeD : Desc TypeD:=
+  {
+    To := Type;
+    denote := denoteTypeD;
+  }.
+
+Notation "a --> b" := (ArrowD a b) (at level 99, right associativity).
+Notation "[ a ]d" := (ListD a).
+
+Check List.fold_left.
+
+Inductive OpD : TypeD -> Type :=
+| EvenD : OpD ( NatD --> BoolD )
+| FoldLeftD :
+    ∀ (A B : TypeD) (f : OpD (A --> B --> A)) (base : denoteTypeD A),
+      OpD ( [ B ]d --> A )
+| MapD :
+    ∀ (t1 t2 : TypeD) (f : OpD (t1 --> t2)),
+      OpD ( [ t1 ]d --> [ t2 ]d )
+.
+
+Fixpoint denote_OpD (d : TypeD) (opD : OpD d) : denoteTypeD d :=
+  match opD with
+  | EvenD         => Nat.even
+  | FoldLeftD f b => fun l => List.fold_left (denote_OpD f) l b
+  | MapD      f   => List.map (denote_OpD f)
+  end.
+
+Global Instance Desc_OpD d : Desc (OpD d) :=
+  {
+    To := ⟦ d ⟧;
+    denote := @denote_OpD d;
+  }.
+
+Definition mapType t1 t2 := (t1 -> t2) -> list t1 -> list t2.
+
+Theorem JustChecking :
+  ∀ A B (f : OpD (A --> B)) l,
+    ⟦ MapD f ⟧ l = List.map ⟦ f ⟧ l.
+Proof.
+  reflexivity.
+Qed.
+
+(*
+Record Δ (D : TypeD) :=
+  {
+    δτ : Type;
+    patch : δτ -> denoteTypeD D -> option ⟦ D ⟧
+  }.
+
+Definition δBoolD : Δ BoolD.
+  apply Build_Δ with (δτ := δAtom.Δ bool).
+  apply δAtom.patch.
+Defined.
+*)
