coq/Diff/Atom.v
@@ -1,0 +1,25 @@
+Set Implicit Arguments.
+
+Inductive Δ (τ : Type) : Type :=
+| Same    :      Δ τ
+| Replace : τ -> Δ τ
+.
+Arguments Same [τ].
+
+Definition patch τ (δ : Δ τ) : τ -> option τ :=
+  match δ with
+  | Same      => Some
+  | Replace r => fun _ => Some r
+  end.
+
+(*
+Global Instance Desc_Δ τ : Desc (Δ τ) :=
+  {
+    To := τ -> τ;
+    denote δ :=
+      match δ with
+      | Same      => id
+      | Replace r => fun _ => r
+      end;
+  }.
+*)
