coq/Diff/List.v
@@ -1,0 +1,48 @@
+Set Implicit Arguments.
+
+From Coq Require Import
+     List
+     Unicode.Utf8
+.
+
+From Chick Require Import
+     Notations
+.
+
+Import ListNotations.
+
+Inductive Δ (τ : Type) (Δτ : Type) : Type :=
+| Insert : ∀ (h  : τ)  (Δt : Δ τ Δτ), Δ τ Δτ
+| Keep   : ∀ (Δt : Δ τ Δτ), Δ τ Δτ
+| Modify : ∀ (Δh : Δτ) (Δt : Δ τ Δτ), Δ τ Δτ
+| Same   : Δ τ Δτ
+.
+Arguments Same [τ Δτ].
+
+Fixpoint patch τ Δτ (patchτ : Δτ -> τ -> option τ)
+         (δ : Δ τ Δτ) : list τ -> option (list τ) :=
+  match δ with
+
+  | Insert h  δt => fun l => cons h <$> patch patchτ δt l
+
+  | Keep δt =>
+    fun l =>
+      match l with
+      | h :: t => cons h <$> patch patchτ δt t
+      | _ => None
+      end
+
+  | Modify δh δt =>
+    fun l =>
+      match l with
+      | []     => None
+      | h :: t =>
+        match (patchτ δh h, patch patchτ δt t) with
+        | (Some h', Some t') => Some (h' :: t')
+        | _ => None
+        end
+      end
+
+  | Same         => Some
+
+  end.
