coq/Syntax/Term.v
@@ -1,0 +1,24 @@
+Set Implicit Arguments.
+
+From Coq Require Import
+     Program
+     String
+     Unicode.Utf8
+.
+
+Definition Variable' := string.
+
+Definition Binder ν := option ν.
+
+Inductive Term (ν : Type) : Type :=
+| App   : ∀ (t1 t2 : Term ν), Term ν
+| Pi    : ∀ (τ1 : Term ν) (b : Binder ν) (τ2 : Term ν), Term ν
+| Type' : Term ν
+| Var   : ∀ (v : ν), Term ν
+.
+Arguments Type' [ν].
+
+Definition VTerm ν := (ν * Term ν)%type.
+Definition VTerms ν := list (VTerm ν).
+Definition BTerm ν := (Binder ν * Term ν)%type.
+Definition BTerms ν := list (BTerm ν).
