coq/Notations.v
@@ -1,0 +1,5 @@
+Set Implicit Arguments.
+
+Notation "f $ x" := (f x) (right associativity, at level 180, only parsing).
+
+Notation "f <$> x" := (option_map f x) (at level 60).
